feat: sponge_squeeze verified

lean/Shars/Verification/SpongeSqueeze.lean
@@ -12,7 +12,7 @@ import Shars.Verification.Utils
 import Shars.Verification.Refinement
 import Shars.Verification.Auxiliary
 import Shars.Verification.KeccakP
-import Shars.Verification.ListIR
+-- import Shars.Verification.ListIR
 
 set_option maxHeartbeats 100000
 attribute [-simp] List.getElem!_eq_getElem?_getD
@@ -22,11 +22,12 @@ open Aeneas
 
 -- attribute [scalar_tac_simps] Nat.pos_of_neZero
 
+/-- The shape of the sponge_squeeze algorithm, operating on bits -/
 def algos.sponge_squeeze.panic_free(r: Nat)[NeZero r](dst s: List Bool)(offset: Nat): List Bool :=
-  assert! s.length ≥ r
+  -- assert! s.length ≥ r
   if offset + r < dst.length then
     let dst' := dst.setSlice! offset (s.take r)
-    let s' := ListIR.list_keccak_p s
+    let s' := IR.keccak_p s
     panic_free r dst' s' (offset + r)
   else
     let nb_left := dst.length - offset
@@ -34,43 +35,123 @@ def algos.sponge_squeeze.panic_free(r: Nat)[NeZero r](dst s: List Bool)(offset: 
 termination_by dst.length - offset
 decreasing_by scalar_decr_tac
 
-def algos.sponge.squeeze.length_panic_free(r: Nat)(dst s: List Bool)(offset: Nat)
+@[simp] theorem algos.sponge.squeeze.length_panic_free(r: Nat)(dst s: List Bool)(offset: Nat)
   (r_pos: r > 0)
-  (r_lt: r < 1600)
-: s.length ≥ r
-→ have: NeZero r := {out := Nat.ne_zero_of_lt r_pos}
+: have: NeZero r := {out := Nat.ne_zero_of_lt r_pos}
   (algos.sponge_squeeze.panic_free r dst s offset).length = dst.length
 := by
-  intro s_big_enough
   unfold algos.sponge_squeeze.panic_free
-  simp only [↓reduceIte, s_big_enough]
+  simp only [↓reduceIte]
   split
   case isTrue h =>
     rw [algos.sponge.squeeze.length_panic_free]
-    all_goals simp [*,le_of_lt]
+    all_goals simp +decide [*, le_of_lt, Spec.b, Spec.w]
   case isFalse h =>
     simp
 termination_by dst.length - offset
 decreasing_by scalar_tac
 
+-- @[simp]
+theorem List.toBits_slice(ls: List (Std.UScalar ty))
+: (ls.slice i j).toBits = ls.toBits.slice (i * ty.numBits) (j * ty.numBits)
+:= by simp only [slice, toBits_take, toBits_drop, Nat.sub_mul]
+
+@[simp]
+theorem List.setSlice!_zero_of_length_le(ls s: List α)
+: ls.length ≤ s.length
+→ ls.setSlice! 0 s = s.take (ls.length)
+:= by intro cond; simp [List.setSlice!, cond]
+
+theorem List.length_slice(ls: List α): (ls.slice a b).length = (b - a) ⊓  (ls.length - a) := by simp [List.slice]
+
+attribute [scalar_tac ls.toBits] List.length_toBits
+attribute [scalar_tac_simps] Std.UScalarTy.numBits
+
+theorem algos.sponge_squeeze.panic_free.extracted_1 (r i : Std.Usize) (dst : Std.Slice Std.U8) (s : StateArray)
+  (r_pos : 0 < (↑r : ℕ))
+
+  (i1 : Std.Usize)
+  (i1_post : (↑i1 : ℕ) = (↑i : ℕ) + (↑r : ℕ))
+  (h : (↑i1 : ℕ) < (↑dst : List Std.U8).length) -- Needed by A and C
+
+  (__discr_1 : Std.Slice Std.U8) (__discr_2 : Std.Slice Std.U8 → Std.Slice Std.U8) -- Needed by ↓ and 2↓
+  (__discr_post_1 : (↑__discr_1 : List Std.U8) = List.slice (↑i : ℕ) (↑i1 : ℕ) (↑dst : List Std.U8)) -- Needed by A
+  (__discr_post_2 : -- Needed by B
+    ∀ (u : Std.Slice Std.U8),
+      u.length = (↑i1 : ℕ) - (↑i : ℕ) →
+        (↑(__discr_2 u) : List Std.U8) = (↑dst : List Std.U8).setSlice! (↑i : ℕ) (↑u : List Std.U8))
+
+  (s2 : Std.Slice Std.U8) -- Needed by ↓
+  (s2_post : s2.toBits = __discr_1.toBits.setSlice! 0 (Std.Array.toBits s)) -- Needed by A
+: (↑i1 : ℕ) ≤ (__discr_2 s2).length := by
+    have: s2.length = r := by scalar_tac -- A
+    have: (__discr_2 s2).length = dst.length := by scalar_tac
+    scalar_tac -- C
+    done
+
+set_option pp.coercions.types true in
+set_option maxHeartbeats 1000000 in
+/-- We prove that the algorithm, under certain preconditions, does not panic -/
+theorem algos.sponge_squeeze.panic_free.refinement(r i d: Std.Usize)
+  (dst: Std.Slice Std.U8)(s: StateArray)
+: (r_bnd: 0 < r.val ∧ r.val < 200)
+→ i ≤ dst.length
+→ dst.length + r.val < Std.Usize.max
+→ d = Std.Usize.ofNatCore dst.length (by have := dst.property; scalar_tac)
+→ let _: NeZero r.val := {out:= Nat.ne_zero_of_lt r_bnd.left}
+  ∃ output,
+  sponge_squeeze_loop r dst s i d = .ok output ∧
+  output.toBits = panic_free (8*r.val) dst.toBits s.toBits (8*i.val)
+:= by
+  rintro ⟨r_pos, r_bnd⟩ i_loop_bnd no_overflow rfl
+  unfold algos.sponge_squeeze_loop panic_free
+  simp [DerefalgosStateArrayArrayU6425.deref, Std.toResult,
+        Std.core.array.Array.index,       Std.core.array.Array.index_mut,
+        Std.core.slice.index.Slice.index, Std.core.slice.index.Slice.index_mut,
+        Aeneas.Std.core.ops.index.Index.index,
+        Std.core.ops.index.IndexSliceInst,
+      ]
+  progress* by simp; scalar_tac
+  · -- have: s2.length = r := by scalar_tac
+    -- have: (__discr_2 s2).length = dst.length := by simp [*]
+    progress as ⟨res, res_post⟩
+    · extract_goal
+    simp [*, le_of_lt]
+    simp_ifs
+    simp only [*, List.toBits_slice, Std.UScalarTy.numBits]
+    rw [List.setSlice!_zero_of_length_le]; case a => simp [List.length_slice]; omega
+    have: (List.slice (i.val * 8) ((i.val + r.val)* 8) dst.toBits).length = 8*r.val := by
+      scalar_tac
+    simp [*, this, IR.keccak_p, Nat.mul_add]
+  · rw [__discr_post_2]
+    case a =>
+      have: s2.toBits.length = dst.toBits.length - 8*i := by simp +arith [*]
+      simpa [Nat.mul_comm 8, ←Nat.sub_mul] using this
+    simp [*]
+    simp_ifs
+    rw [List.setSlice!_zero_of_length_le]; case a => simp; scalar_tac
+    simp [Nat.mul_comm 8]
+termination_by dst.length - i.val
+decreasing_by scalar_decr_tac
+
 attribute [local scalar_tac_simps] not_le in
-def ListIR.sponge.squeeze(d: Nat)(r: Nat)[NeZero r](dst s: List Bool): List Bool :=
+/-- This is a representation of squeeze which is closer to the Spec -/
+def IR.squeeze(d: Nat)(r: Nat)[NeZero r](dst s: List Bool): List Bool :=
   if d ≤ dst.length then
     dst.take d
   else
-    squeeze d r (dst ++ s.setWidth r) (ListIR.list_keccak_p s)
+    squeeze d r (dst ++ s.setWidth r) (IR.keccak_p s)
 termination_by d - dst.length
 decreasing_by scalar_decr_tac
 
 @[simp]
-theorem ListIR.sponge.length_squeeze(d: Nat)(r: Nat)[NeZero r](dst s: List Bool)
+theorem IR.length_squeeze(d: Nat)(r: Nat)[NeZero r](dst s: List Bool)
 : (squeeze d r dst s).length = d
 := by
   unfold squeeze
   split
   case isTrue h => simp [h]
-  case isFalse h =>
-    rw [ListIR.sponge.length_squeeze]
+  case isFalse h => rw [IR.length_squeeze]
 termination_by d - dst.length
 decreasing_by scalar_decr_tac
 
@@ -91,32 +172,33 @@ private theorem List.getElem!_setSlice!_eq_ite[Inhabited α](ls slice: List α)(
 
 attribute [local simp_lists_simps] List.getElem!_take_eq_ite in
 set_option maxHeartbeats 1000000 in
+/-- We show that the Spec-similar function is equivalent to the algo-similar function -/
 theorem algos.sponge_squeeze.panic_free.spec(r: Nat)
   (r_bnd: 0 < r ∧ r < 1600)
   (dst s: List Bool)(offset : Nat)
 : s.length = 1600
 → offset ≤ dst.length
 → have : NeZero r := {out := Nat.ne_zero_of_lt r_bnd.left}
-  panic_free r dst s offset = ListIR.sponge.squeeze dst.length r (dst.take offset) s
+  panic_free r dst s offset = IR.squeeze dst.length r (dst.take offset) s
 := by
   obtain ⟨r_pos, r_lt⟩ := r_bnd
   intro len_s offset_idx
   simp
-  unfold panic_free ListIR.sponge.squeeze
+  unfold panic_free IR.squeeze
   simp [*, le_of_lt]
   split
   case isTrue next_offset_lt =>
     simp_ifs
     rw [spec r]
-    all_goals simp [*, le_of_lt]
+    all_goals simp +decide [*, le_of_lt]
     congr 1
-    ext i
-    · simp [*, le_of_lt]
+    apply List.ext_getElem <;> simp [*, le_of_lt, ←getElem!_pos]
+    intro i i_lt
+    simp [List.setSlice!, *]
     assume i < offset + r; case otherwise => simp_lists
     simp_lists [List.getElem!_take_eq_ite, List.getElem!_setSlice!_eq_ite]
-    simp_ifs
   case isFalse end_of_processing =>
-    unfold ListIR.sponge.squeeze
+    unfold IR.squeeze
     simp_ifs
     split
     · simp [‹offset = dst.length›', List.setSlice!]
@@ -142,97 +224,42 @@ theorem dite_eq_then {α : Sort u} (c : Prop) [h : Decidable c] (t : c → α) (
 theorem dite_eq_else {α : Sort u} (c : Prop) [h : Decidable c] (t : c → α) (e : ¬c → α) (h : ¬ c) :
   dite c t e = e h := by simp only [↓reduceDIte, h]
 
-#check Std.Usize.ofNatCore
+@[simp]
+theorem Vector.toList_setWidth[Inhabited α](v: Vector α n)(m: Nat)
+: (v.setWidth m).toList = v.toList.setWidth m
+:= by simp [Vector.setWidth, List.setWidth]
 
-set_option maxHeartbeats 100000000 in
-set_option maxRecDepth 1000000 in
--- set_option trace.meta.Tactic.simp true in
-theorem algos.sponge_squeeze.panic_free.refinement(r i d: Std.Usize)
-  (dst: Std.Slice Bool)(s: Aeneas.Std.Array Bool 1600#usize)
-: (r_bnd: 0 < r.val ∧ r.val < 1600)
-→ i ≤ dst.length
-→ dst.length + r.val < Std.Usize.max
-→ d = Std.Usize.ofNatCore dst.length (by have := dst.property; scalar_tac)
-→ let _: NeZero r.val := {out:= Nat.ne_zero_of_lt r_bnd.left}
-  ∃ output,
-  sponge_squeeze_loop r dst s i d = .ok output ∧
-  output.val = panic_free r.val dst.val s.val i.val
+def IR.squeeze.refinement(r: { x // 0 < x ∧ x < Spec.b 6 })
+    (Z: Spec.Bitstring m)
+    (S: Spec.Bitstring (Spec.b 6))
+: have: NeZero r.val := {out:= by omega}
+  (Spec.sponge.squeeze (d := d) (f := Spec.Keccak.P 6 24) r Z S).toList =
+  (squeeze d r Z.toList S.toList)
 := by
-  rintro r_bnd i_idx no_overflow rfl
-  unfold algos.sponge_squeeze_loop panic_free
-  let* ⟨ i1, i1_post ⟩ ← Std.Usize.add_spec
-  split
-  . simp [Std.core.slice.index.Slice.index_mut, Std.core.slice.index.SliceIndexRangeUsizeSlice.index_mut, *]
-    simp_ifs
-    simp [Std.core.array.Array.index, Std.core.ops.index.IndexSliceInst, Std.core.slice.index.Slice.index, Std.core.slice.index.SliceIndexRangeUsizeSlice.index, Std.Array.to_slice, *]
-    simp_ifs
-    simp [Std.core.slice.Slice.copy_from_slice, List.slice, Std.Slice.len, *]
-    simp_ifs
-    simp [*, le_of_lt]
-    let* ⟨ s4, s4_post ⟩ ← keccak_p.spec'
-    let* ⟨ s4, s4_post ⟩ ← refinement
-    simp [*]
-  . let* ⟨ nb_left, nb_left_post ⟩ ← Aeneas.Std.Usize.sub_spec'
-    simp at nb_left_post
-    simp [Std.core.slice.index.Slice.index_mut, Std.core.slice.index.SliceIndexRangeFromUsizeSlice.index_mut, *]
-    simp [Std.core.array.Array.index, Std.core.ops.index.IndexSliceInst, Std.core.slice.index.Slice.index, Std.core.slice.index.SliceIndexRangeUsizeSlice.index, Std.Array.to_slice, *]
-    simp_ifs
-    simp [Std.core.slice.Slice.copy_from_slice, List.slice, Std.Slice.len, *, Nat.min_def, List.length_drop]
-    simp_ifs
-    simp [*]
-    simp_ifs
-    simp [List.setSlice!, *]
-    simp_lists
-termination_by dst.length - i
-decreasing_by scalar_decr_tac
-
-attribute [local simp_lists_simps] List.getElem!_take_eq_ite in
-set_option maxRecDepth 1000000 in
-def ListIR.sponge.squeeze.refinement(r: Nat) [NeZero r]
-    (Z: BitVec m)
-    (S: BitVec (Spec.b 6))
-: Spec.sponge.squeeze (d := d) (f := Spec.Keccak.P 6 24) r Z S =
-  (squeeze d r Z.toList S.toList).toBitVec.cast (by simp)
-:= by
-  refine BitVec.toList_inj ?_
-
-  simp
   unfold squeeze Spec.sponge.squeeze
   simp
   split
   case isTrue base_case =>
-    simp [base_case, BitVec.toList]
-    ext i
-    · simp [*]
-    simp_lists
-    simp
-    assume i < d
-    case otherwise h => simp [h]
-    simp [*, ‹i < m›']
+    simp [base_case, Vector.setWidth]
   case isFalse _ =>
-    rw [ListIR.sponge.squeeze.refinement]
-    simp [ListIR.list_keccak_p, BitVec.toBitVec_toList]
-    congr
-    simp [BitVec.toList_setWidth]
+    rw [IR.squeeze.refinement]
+    simp [IR.keccak_p, List.toStateArray]
 termination_by d - m
 decreasing_by scalar_decr_tac
 
-
+/-- The final theorem, putting everything together -/
 theorem algos.sponge_squeeze.spec(r: Std.Usize)
-  (dst: Std.Slice Bool)(s: Aeneas.Std.Array Bool 1600#usize)
-: (r_bnd: 0 < r.val ∧ r.val < 1600)
+  (dst: Std.Slice Std.U8)(s: StateArray)
+: (r_bnd: 0 < r.val ∧ r.val < 200)
 → dst.length + r.val < Std.Usize.max
-→ let _: NeZero r.val := {out:= Nat.ne_zero_of_lt r_bnd.left}
+→ have _: NeZero r.val := {out:= Nat.ne_zero_of_lt r_bnd.left}
   ∃ output,
   sponge_squeeze r dst s = .ok output ∧
-  output.val = ListIR.sponge.squeeze dst.length r [] s.val
+  output.toBits = IR.squeeze dst.toBits.length (8*r) [] s.toBits
 := by
   intros
   rw [sponge_squeeze]
   progress with algos.sponge_squeeze.panic_free.refinement as ⟨res, res_post⟩
   rw [res_post]
   rw [algos.sponge_squeeze.panic_free.spec]
-  · simp
-  · assumption
-  · simp
-  · simp
+  all_goals simp [*]; try omega
